src/proof/kubernetes_model/tx/update.v
@@ -15,7 +15,9 @@ Lemma wp_State__updateTx_au γ l kind namespace i kobj :
   ∀ Φ,
     is_pkg_init apimodel ∗
     is_kubernetes γ l ∗
-    "%Hvalid" ∷ ⌜ KObjectV.valid kobj ⌝ ∗
+    "%Hvalid" ∷ ⌜ KObjectV.valid_named_create kind namespace kobj ⌝ ∗
+    "%Huid_nonempty" ∷
+      ⌜ (KObjectV.objectmeta kobj).(ObjectMetaV.UID') ≠ ""%go ⌝ ∗
     "%Hkind_matches" ∷ ⌜ kind = KObjectV.kind kobj ⌝ ∗
     "%Hns_matches" ∷ ⌜ namespace = (KObjectV.objectmeta kobj).(ObjectMetaV.Namespace') ⌝ ∗
     "Hdeepown_i" ∷ KObjectV.deepown_i i kobj 1 ∗
@@ -84,8 +86,9 @@ Proof.
   wp_apply (wp_GetName_deepown with "[$Hdeepown_metadata]").
   iIntros "Hdeepown_metadata". wp_auto.
   assert (ObjectMetaV.Name' (KObjectV.objectmeta kobj) ≠ ""%go) as Hname_not_empty.
-  { destruct Hvalid as (_ & _ & Hmeta & _).
-    eapply ObjectMetaV.valid_name_nonempty_of_valid. done. }
+  { pose proof Hvalid as Hvalid_copy.
+    destruct Hvalid_copy as (_ & _ & Hmeta & _).
+    unfold ObjectMetaV.valid_named_create in Hmeta. tauto. }
   rewrite bool_decide_false //. wp_auto.
   set key := {|
     KKey.Kind' := kind;
@@ -141,9 +144,19 @@ Proof.
     (ObjectMetaV.ResourceVersion' (KObjectV.objectmeta existing_kobj))) as
     Hexisting_rv_valid.
   { destruct Hvalid_existing as (_ & Hrv_valid & _). done. }
-  assert (KObjectV.valid kobj_rv) as Hvalid_rv.
+  assert (KObjectV.valid_named_create kind namespace kobj_rv)
+    as Hvalid_create_rv.
   { subst kobj_rv kmeta_rv.
-    apply valid_update_objectmeta_set_resource_version; done. }
+    rewrite /KObjectV.valid_named_create
+      KObjectV.kind_update_objectmeta KObjectV.typemeta_update_objectmeta
+      objectmeta_update_objectmeta KObjectV.spec_update_objectmeta.
+    destruct Hvalid as (Hkind & Htypemeta & Hmeta & Hspec).
+    split_and!; done. }
+  assert ((KObjectV.objectmeta kobj_rv).(ObjectMetaV.UID') ≠ ""%go)
+    as Huid_nonempty_rv.
+  { subst kobj_rv kmeta_rv.
+    rewrite objectmeta_update_objectmeta /=.
+    exact Huid_nonempty. }
   assert (kind = KObjectV.kind kobj_rv) as Hkind_matches_rv.
   { subst kobj_rv. rewrite KObjectV.kind_update_objectmeta. done. }
   assert (namespace = ObjectMetaV.Namespace' (KObjectV.objectmeta kobj_rv)) as
@@ -153,6 +166,10 @@ Proof.
   iFrame "#".
   iFrame "Hdeepown_i_copy".
   iSplit; first done.
+  iSplit; first done.
+  iSplit.
+  { iPureIntro. subst kobj_rv kmeta_rv.
+    rewrite objectmeta_update_objectmeta /=. exact Hexisting_rv_valid. }
   iSplit; first done.
   iSplit; first done.
   iMod "Hau" as (key1 uid1 kmeta1 kspec1) "[Hau_pre Hclose]".
@@ -224,7 +241,9 @@ Qed.
 Lemma wp_State__updateTx γ l kind namespace i kobj key uid kmeta kspec :
   {{{ is_pkg_init apimodel ∗
       "#Hisk" ∷ is_kubernetes γ l ∗
-      "%Hvalid" ∷ ⌜ KObjectV.valid kobj ⌝ ∗
+      "%Hvalid" ∷ ⌜ KObjectV.valid_named_create kind namespace kobj ⌝ ∗
+      "%Huid_nonempty" ∷
+        ⌜ (KObjectV.objectmeta kobj).(ObjectMetaV.UID') ≠ ""%go ⌝ ∗
       "%Hkind_matches" ∷ ⌜ kind = KObjectV.kind kobj ⌝ ∗
       "%Hns_matches" ∷ ⌜ namespace = (KObjectV.objectmeta kobj).(ObjectMetaV.Namespace') ⌝ ∗
       "%Hkey_eq" ∷ ⌜ key = KObjectV.key kobj ⌝ ∗
@@ -277,7 +296,9 @@ Qed.
 Lemma wp_State__PodUpdateTx γ l namespace pod_l pod key uid kmeta kspec :
   {{{ is_pkg_init apimodel ∗
       "#Hisk" ∷ is_kubernetes γ l ∗
-      "%Hvalid" ∷ ⌜ PodV.valid pod ⌝ ∗
+      "%Hvalid" ∷ ⌜ PodV.valid_named_create namespace pod ⌝ ∗
+      "%Huid_nonempty" ∷
+        ⌜ pod.(PodV.ObjectMeta').(ObjectMetaV.UID') ≠ ""%go ⌝ ∗
       "%Hns_matches" ∷
         ⌜ namespace = pod.(PodV.ObjectMeta').(ObjectMetaV.Namespace') ⌝ ∗
       "%Hkey_eq" ∷ ⌜ key = PodV.key pod ⌝ ∗
@@ -323,12 +344,14 @@ Proof.
       (KObjectV.Pod pod) 1)
     with "[Hdeepown_l]" as "Hdeepown_i".
   { iExists pod_l. iSplit; [done|]. iFrame. }
+  assert (KObjectV.valid_named_create PodV.kind namespace
+      (KObjectV.Pod pod)) as Hvalid_kobj.
+  { rewrite /KObjectV.valid_named_create /=. split; done. }
   wp_apply (wp_State__updateTx γ l PodV.kind namespace
     (interface.mk (go.PointerType v1.Pod) #pod_l)
     (KObjectV.Pod pod) key uid kmeta kspec
     with "[$Hinit $Hisk $Hdeepown_i $Hown_meta_frag $Hown_spec_frag]").
   { iPureIntro.
-    rewrite KObjectV.valid_eq_valid2 /=.
     split_and!; done. }
   iIntros (i' kobj') "Hpost". iNamed "Hpost".
   destruct kobj' as [pod'|rs'|pvc'|sts']; try done.
